Propageted changes to the proof, looks much better

theories/L6_PCPS/Heap/closure_conversion_correct.v
@@ -24,62 +24,38 @@ Module ClosureConversionCorrect (H : Heap).
   (** Invariant about the free variables *) 
   Definition FV_inv (k j : nat) (IP : GIInv) (P : GInv) (b : Inj)
              (rho1 : env) (H1 : heap block) (rho2 : env) (H2 : heap block)
-             (c : cTag) (Scope Funs : Ensemble var) (Γ : var) (FVs : list var) : Prop :=
+             (c : cTag) (Scope : Ensemble var) (Γ : var) (FVs : list var) : Prop :=
     exists (vs : list value) (l : loc),
       M.get Γ rho2 = Some (Loc l) /\
       get l H2 = Some (Constr c vs) /\
-      Forall2_P (Scope :|: Funs)
+      Forall2_P Scope
                 (fun (x : var) (v2 : value)  =>
                    exists v1, M.get x rho1 = Some v1 /\
                          Res (v1, H1) ≺ ^ ( k ; j ; IP ; P ; b) Res (v2, H2)) FVs vs.
+
   
-  (** Invariant about the functions in the current function definition *)
-  Definition Fun_inv (k j : nat) (IP : GIInv) (P : GInv) (b : Inj)
-             (rho1 : env) (H1 : heap block) (rho2 : env) (H2 : heap block)
-             (Scope Funs : Ensemble var) : Prop :=
-    (* (exists f, f \in Funs) /\ *)
-    forall (f : var),
-    ~ f \in Scope ->
-    f \in Funs ->
-    exists lf1 lf2,
-      M.get f rho1 = Some lf1 /\ 
-      M.get f rho2 = Some lf2 /\
-      Res (lf1, H1) ≺ ^ ( k ; j ; IP ; P ; b) Res (lf2, H2).
-  
-  (** Versions without the logical relation. Useful when we're only interested in other invariants. *)
+  (** Version without the logical relation. Useful when we're only interested in other invariants. *)
   
   (** Invariant about the free variables *) 
   Definition FV_inv_weak (rho1 : env) (rho2 : env) (H2 : heap block)
-             (c : cTag) (Scope Funs : Ensemble var) (Γ : var) (FVs : list var) : Prop :=
+             (c : cTag) (Scope : Ensemble var) (Γ : var) (FVs : list var) : Prop :=
     exists (vs : list value) (l : loc),
       M.get Γ rho2 = Some (Loc l) /\
       get l H2 = Some (Constr c vs) /\
-      Forall2_P (Scope :|: Funs)
+      Forall2_P Scope
                 (fun (x : var) (v2 : value)  =>
                    exists v1, M.get x rho1 = Some v1) FVs vs.
   
-  (** Invariant about the functions in the current function definition *)
-  Definition Fun_inv_weak (rho1 : env) (H1 : heap block) (rho2 : env) (H2 : heap block)
-             (Scope Funs : Ensemble var) : Prop :=
-    (* (exists f, f \in Funs \\ Scope) /\ *)
-    forall (f : var),
-      ~ f \in Scope ->
-      f \in Funs  ->    
-      exists lf1 lf2,
-        M.get f rho1 = Some lf1 /\ 
-        M.get f rho2 = Some lf2.
   
   (** * Lemmas about [FV_inv] *)
 
   Require Import Logic.ClassicalFacts.
-
-  Axiom excluded_middle : excluded_middle. (* Get rid of this at some point *)
   
   Lemma FV_inv_image_post (k j : nat) (GII : GIInv) (GI : GInv) (b : Inj)
              (rho1 : env) (H1 : heap block) (rho2 : env) (H2 : heap block)
-             (c : cTag) (Scope Funs : Ensemble var) (Γ : var) (FVs : list var) :
-    FV_inv k j GII GI b rho1 H1 rho2 H2 c Scope Funs Γ FVs ->    
-    image b ((post H1 ^ j) (env_locs rho1 (FromList FVs \\ (Scope :|: Funs)))) \subset
+             (c : cTag) (Scope : Ensemble var) `{Decidable _ Scope} (Γ : var) (FVs : list var) :
+    FV_inv k j GII GI b rho1 H1 rho2 H2 c Scope Γ FVs ->    
+    image b ((post H1 ^ j) (env_locs rho1 (FromList FVs \\ Scope))) \subset
     (post H2 ^ j) (post H2 (env_locs rho2 ([set Γ]))).
   Proof with (now eauto with Ensembles_DB).
     intros (vs & l & Hget1 & Hget2 & Hall).
@@ -95,30 +71,30 @@ Module ClosureConversionCorrect (H : Heap).
       rewrite post_n_Empty_set, image_Empty_set...
     - rewrite proper_post_n;
       [| rewrite FromList_cons, Setminus_Union_distr, env_locs_Union
-         ; try reflexivity ]. 
-      destruct (excluded_middle ((Scope :|: Funs) x)).
+         ; try reflexivity ].
+      simpl. 
+      rewrite !post_n_Union, image_Union.
+      eapply Included_Union_compat; [| eassumption ]. 
+      destruct H as [Hdec]. destruct (Hdec x). 
       + rewrite proper_post_n;
-        [| rewrite Setminus_Included_Empty_set, env_locs_Empty_set,
-           Union_Empty_set_neut_l; try reflexivity ].
-        eapply Included_trans. eassumption.
-        eapply post_n_set_monotonic. simpl...
+        [| rewrite Setminus_Included_Empty_set, env_locs_Empty_set; try reflexivity ].
+        rewrite post_n_Empty_set, image_Empty_set...
         eapply Singleton_Included. eassumption.
-      +rewrite proper_post_n;
-        [| rewrite Setminus_Disjoint; try reflexivity ].
-       simpl. rewrite !post_n_Union, image_Union.
-       eapply Included_Union_compat; eauto.
-       destruct (H H0) as [v1 [Hget1 Hres]].
-       rewrite proper_post_n; 
+      + rewrite proper_post_n;
+         [| rewrite Setminus_Disjoint; try reflexivity ].
+        simpl.
+        destruct (H0 n) as [v1 [Hget1 Hres]].
+        rewrite proper_post_n; 
         [| rewrite env_locs_Singleton; eauto; reflexivity ].
       eapply cc_approx_val_image_eq. eassumption.
       eapply Disjoint_Singleton_l; eauto.
   Qed.
-
+  
   Lemma FV_inv_image_post_eq (k j : nat) (GII : GIInv) (GI : GInv) (b : Inj)
              (rho1 : env) (H1 : heap block) (rho2 : env) (H2 : heap block)
-             (c : cTag) (Scope Funs : Ensemble var) (Γ : var) (FVs : list var) :
-    FV_inv k j GII GI b rho1 H1 rho2 H2 c Scope Funs Γ FVs ->
-    Disjoint _ (FromList FVs) (Scope :|: Funs) ->
+             (c : cTag) (Scope : Ensemble var) `{Decidable _ Scope} (Γ : var) (FVs : list var) :
+    FV_inv k j GII GI b rho1 H1 rho2 H2 c Scope Γ FVs ->
+    Disjoint _ (FromList FVs) Scope ->
     image b ((post H1 ^ j) (env_locs rho1 (FromList FVs))) <-->
     (post H2 ^ j) (post H2 (env_locs rho2 ([set Γ]))).
   Proof with (now eauto with Ensembles_DB).
@@ -126,7 +102,7 @@ Module ClosureConversionCorrect (H : Heap).
     - eapply Included_trans.
       eapply image_monotonic. eapply post_n_set_monotonic.
       rewrite <- (Setminus_Disjoint (FromList FVs)); try eassumption.
-      reflexivity. eapply FV_inv_image_post. eassumption.
+      reflexivity. eapply FV_inv_image_post; eassumption.
     - destruct Hfv as (vs & l & Hget1 & Hget2 & Hall).
       eapply Included_trans; [ eapply post_n_set_monotonic;
                                rewrite env_locs_Singleton; eauto; simpl;
@@ -134,9 +110,9 @@ Module ClosureConversionCorrect (H : Heap).
       clear Hget1 Hget2.
       induction Hall.
       * simpl. rewrite post_n_Empty_set...
-      * assert (Hneq : ~ (Scope :|: Funs) x).
+      * assert (Hneq : ~ (Scope x)).
         { intros Hc. eapply Hd. constructor; eauto. constructor; eauto. }
-        destruct (H Hneq) as [v1 [Hget1 Hres]].
+        destruct (H0 Hneq) as [v1 [Hget1 Hres]].
         eapply Included_trans;
         [| eapply image_monotonic; eapply post_n_set_monotonic;
            rewrite FromList_cons, env_locs_Union, env_locs_Singleton; eauto; reflexivity ]. 
@@ -149,10 +125,10 @@ Module ClosureConversionCorrect (H : Heap).
   
   Lemma FV_inv_j_monotonic (k j' j : nat) (GII : GIInv) (GI : GInv) (b : Inj)
         (rho1 : env) (H1 : heap block) (rho2 : env) (H2 : heap block)
-        (c : cTag) (Scope Funs : Ensemble var) (Γ : var) (FVs : list var) :
-    FV_inv k j GII GI b rho1 H1 rho2 H2 c Scope Funs Γ FVs ->
+        (c : cTag) (Scope : Ensemble var) (Γ : var) (FVs : list var) :
+    FV_inv k j GII GI b rho1 H1 rho2 H2 c Scope Γ FVs ->
     j' <= j ->
-    FV_inv k j' GII GI b rho1 H1 rho2 H2 c Scope Funs Γ FVs.
+    FV_inv k j' GII GI b rho1 H1 rho2 H2 c Scope Γ FVs.
   Proof.
     intros Hfv Hlt. 
     destruct Hfv as (v & vs & Hget1 & Hget2 & Hall).
@@ -165,10 +141,10 @@ Module ClosureConversionCorrect (H : Heap).
 
   Lemma FV_inv_monotonic (k k' j : nat) (GII : GIInv) (GI : GInv) (b : Inj)
         (rho1 : env) (H1 : heap block) (rho2 : env) (H2 : heap block)
-        (c : cTag) (Scope Funs : Ensemble var) (Γ : var) (FVs : list var) :
-    FV_inv k j GII GI b rho1 H1 rho2 H2 c Scope Funs Γ FVs ->
+        (c : cTag) (Scope : Ensemble var) (Γ : var) (FVs : list var) :
+    FV_inv k j GII GI b rho1 H1 rho2 H2 c Scope Γ FVs ->
     k' <= k ->
-    FV_inv k' j GII GI b rho1 H1 rho2 H2 c Scope Funs Γ FVs.
+    FV_inv k' j GII GI b rho1 H1 rho2 H2 c Scope Γ FVs.
   Proof.
     intros Hfv Hlt. 
     destruct Hfv as (v & vs & Hget1 & Hget2 & Hall).
@@ -181,45 +157,44 @@ Module ClosureConversionCorrect (H : Heap).
     
   Lemma FV_inv_image_reach_n (k j : nat) (GII : GIInv) (GI : GInv) (b : Inj)
              (rho1 : env) (H1 : heap block) (rho2 : env) (H2 : heap block)
-             (c : cTag) (Scope Funs : Ensemble var) (Γ : var) (FVs : list var) :
-    FV_inv k j GII GI b rho1 H1 rho2 H2 c Scope Funs Γ FVs ->    
-    image b (reach_n H1 j (env_locs rho1 (FromList FVs \\ (Scope :|: Funs)))) \subset
+             (c : cTag) (Scope : Ensemble var) `{Decidable _ Scope} (Γ : var) (FVs : list var) :
+    FV_inv k j GII GI b rho1 H1 rho2 H2 c Scope Γ FVs ->    
+    image b (reach_n H1 j (env_locs rho1 (FromList FVs \\ Scope))) \subset
     (reach_n H2 j (post H2 (env_locs rho2 ([set Γ])))).
   Proof.
     intros Hfv. 
     intros l' [l [[m [Hm Hr]] Hin]].
     eapply FV_inv_j_monotonic in Hfv; eauto.
-    eexists m. split; eauto. eapply FV_inv_image_post. eassumption.
+    eexists m. split; eauto. eapply FV_inv_image_post; try eassumption.
     eexists; split; eauto.
-
   Qed.
 
   Lemma FV_inv_image_reach (k : nat) (GII : GIInv) (GI : GInv) (b : Inj)
              (rho1 : env) (H1 : heap block) (rho2 : env) (H2 : heap block)
-             (c : cTag) (Scope Funs : Ensemble var) (Γ : var) (FVs : list var) :
-    (forall j, FV_inv k j GII GI b rho1 H1 rho2 H2 c Scope Funs Γ FVs) ->    
-    image b (reach' H1 (env_locs rho1 (FromList FVs \\ (Scope :|: Funs)))) \subset
+             (c : cTag) (Scope : Ensemble var) `{Decidable _ Scope} (Γ : var) (FVs : list var) :
+    (forall j, FV_inv k j GII GI b rho1 H1 rho2 H2 c Scope Γ FVs) ->    
+    image b (reach' H1 (env_locs rho1 (FromList FVs \\ Scope))) \subset
     (reach' H2 (post H2 (env_locs rho2 ([set Γ])))).
   Proof.
     intros Hfv.
     intros l' [l [[m [Hm Hr]] Heq]].
-    eexists m. split; eauto. eapply FV_inv_image_post. eauto.
+    eexists m. split; eauto. eapply FV_inv_image_post; eauto.
     eexists; split; eauto.
   Qed.
 
   Lemma FV_inv_image_reach_n_eq (k j : nat) (GII : GIInv) (GI : GInv) (b : Inj)
              (rho1 : env) (H1 : heap block) (rho2 : env) (H2 : heap block)
-             (c : cTag) (Scope Funs : Ensemble var) (Γ : var) (FVs : list var) :
-    FV_inv k j GII GI b rho1 H1 rho2 H2 c Scope Funs Γ FVs ->
-    Disjoint _ (FromList FVs) (Scope :|: Funs) ->
+             (c : cTag) (Scope : Ensemble var) `{Decidable _ Scope} (Γ : var) (FVs : list var) :
+    FV_inv k j GII GI b rho1 H1 rho2 H2 c Scope Γ FVs ->
+    Disjoint _ (FromList FVs) Scope ->
     image b (reach_n H1 j (env_locs rho1 (FromList FVs))) <-->
     reach_n H2 j (post H2 (env_locs rho2 ([set Γ]))).
   Proof.
     intros Hfv. split.
     - intros l' [l [[m [Hm Hr]] Hin]].
       eapply FV_inv_j_monotonic in Hfv; eauto.
-      eexists m. split; eauto. eapply FV_inv_image_post_eq. eassumption.
-      eassumption. eexists; split; eauto.
+      eexists m. split; eauto. eapply FV_inv_image_post_eq; try eassumption.
+      eexists; split; eauto.
     - intros l' [m [Hm Hr]].
       eapply FV_inv_j_monotonic in Hfv; eauto.
       eapply FV_inv_image_post_eq in Hr; eauto.
@@ -229,9 +204,9 @@ Module ClosureConversionCorrect (H : Heap).
 
   Lemma FV_inv_image_reach_eq (k : nat) (GII : GIInv) (GI : GInv) (b : Inj)
              (rho1 : env) (H1 : heap block) (rho2 : env) (H2 : heap block)
-             (c : cTag) (Scope Funs : Ensemble var) (Γ : var) (FVs : list var) :
-    (forall j, FV_inv k j GII GI b rho1 H1 rho2 H2 c Scope Funs Γ FVs) ->
-    Disjoint _ (FromList FVs) (Scope :|: Funs) ->
+             (c : cTag) (Scope : Ensemble var) `{Decidable _ Scope} (Γ : var) (FVs : list var) :
+    (forall j, FV_inv k j GII GI b rho1 H1 rho2 H2 c Scope Γ FVs) ->
+    Disjoint _ (FromList FVs) Scope ->
     image b (reach' H1 (env_locs rho1 (FromList FVs))) <-->
     (reach' H2 (post H2 (env_locs rho2 ([set Γ])))).
   Proof.
@@ -245,22 +220,22 @@ Module ClosureConversionCorrect (H : Heap).
       eexists; split; eauto.
   Qed.
   
-  Lemma FV_inv_weak_in_FV_inv k j P1 P2 rho1 H1 rho2 H2 β c Scope Funs Γ FVs :
-    FV_inv k j P1 P2 β rho1 H1 rho2 H2 c Scope Funs Γ FVs ->
-    FV_inv_weak rho1 rho2 H2 c Scope Funs Γ FVs.
+  Lemma FV_inv_weak_in_FV_inv k j P1 P2 rho1 H1 rho2 H2 β c Scope Γ FVs :
+    FV_inv k j P1 P2 β rho1 H1 rho2 H2 c Scope Γ FVs ->
+    FV_inv_weak rho1 rho2 H2 c Scope Γ FVs.
   Proof.
     intros (x1 & x2  & Hget1 & Hget2 & Hall).
     repeat eexists; eauto.
     eapply Forall2_P_monotonic_strong; [| eassumption ].
-    now firstorder.
+    intros ? ? ? ? ? [? [? ? ]]. eexists; eauto.
   Qed.
 
   Lemma FV_inv_set_not_in_FVs_l (k j : nat) (GII : GIInv) (GI : GInv) (b : Inj)
         (rho1 : env) (H1 : heap block) (rho2 : env) (H2 : heap block)
-        (c : cTag) (Scope Funs : Ensemble var) (Γ : var) (FVs : list var) x v  :
-    FV_inv k j GII GI b rho1 H1 rho2 H2 c Scope Funs Γ FVs ->
-    ~ x \in (FromList FVs \\ (Scope :|: Funs)) ->
-    FV_inv k j GII GI b (M.set x v rho1) H1 rho2 H2 c Scope Funs Γ FVs.
+        (c : cTag) (Scope : Ensemble var) (Γ : var) (FVs : list var) x v  :
+    FV_inv k j GII GI b rho1 H1 rho2 H2 c Scope Γ FVs ->
+    ~ x \in (FromList FVs \\ Scope) ->
+    FV_inv k j GII GI b (M.set x v rho1) H1 rho2 H2 c Scope Γ FVs.
   Proof.
     intros (x1 & x2 & Hget1 & Hget2 & Hall).
     repeat eexists; eauto.
@@ -273,10 +248,10 @@ Module ClosureConversionCorrect (H : Heap).
 
   Lemma FV_inv_set_not_in_FVs_r (k j : nat) (GII : GIInv) (GI : GInv) (b : Inj)
         (rho1 : env) (H1 : heap block) (rho2 : env) (H2 : heap block)
-        (c : cTag) (Scope Funs : Ensemble var) (Γ : var) (FVs : list var) x v  :
-    FV_inv k j GII GI b rho1 H1 rho2 H2 c Scope Funs Γ FVs ->
+        (c : cTag) (Scope : Ensemble var) (Γ : var) (FVs : list var) x v  :
+    FV_inv k j GII GI b rho1 H1 rho2 H2 c Scope Γ FVs ->
     x <> Γ ->
-    FV_inv k j GII GI b rho1 H1 (M.set x v rho2) H2 c Scope Funs Γ FVs.
+    FV_inv k j GII GI b rho1 H1 (M.set x v rho2) H2 c Scope Γ FVs.
   Proof.
     intros (x1 & x2 & Hget1 & Hget2 & Hall).
     repeat eexists; eauto.
@@ -285,11 +260,11 @@ Module ClosureConversionCorrect (H : Heap).
   
   Lemma FV_inv_set_not_in_FVs (k j : nat) (GII : GIInv) (GI : GInv) (b : Inj)
         (rho1 : env) (H1 : heap block) (rho2 : env) (H2 : heap block)
-        (c : cTag) (Scope Funs : Ensemble var) (Γ : var) (FVs : list var) x y v v'  :
-    FV_inv k j GII GI b rho1 H1 rho2 H2 c Scope Funs Γ FVs ->
-    ~ x \in (FromList FVs \\ (Scope :|: Funs)) ->
+        (c : cTag) (Scope : Ensemble var) (Γ : var) (FVs : list var) x y v v'  :
+    FV_inv k j GII GI b rho1 H1 rho2 H2 c Scope Γ FVs ->
+    ~ x \in (FromList FVs \\ Scope) ->
     y <> Γ ->
-    FV_inv k j GII GI b (M.set x v rho1) H1 (M.set y v' rho2) H2 c Scope Funs Γ FVs.
+    FV_inv k j GII GI b (M.set x v rho1) H1 (M.set y v' rho2) H2 c Scope Γ FVs.
   Proof.
     intros. eapply FV_inv_set_not_in_FVs_r; eauto.
     eapply FV_inv_set_not_in_FVs_l; eauto.
@@ -299,15 +274,15 @@ Module ClosureConversionCorrect (H : Heap).
   (** [FV_inv] is heap monotonic  *)
   Lemma FV_inv_heap_mon (k j : nat) (GII : GIInv) (GI : GInv) (b : Inj)
         (rho1 : env) (H1 H1' : heap block) (rho2 : env) (H2 H2' : heap block)
-        (c : cTag) (Scope Funs : Ensemble var) (Γ : var) (FVs : list var) :
-    well_formed (reach' H1 (env_locs rho1 (FromList FVs \\ (Scope :|: Funs)))) H1 ->
+        (c : cTag) (Scope : Ensemble var) (Γ : var) (FVs : list var) :
+    well_formed (reach' H1 (env_locs rho1 (FromList FVs \\ Scope))) H1 ->
     well_formed (reach' H2 (env_locs rho2 [set Γ])) H2 ->
-    env_locs rho1 (FromList FVs \\ (Scope :|: Funs)) \subset dom H1 ->
+    env_locs rho1 (FromList FVs \\ Scope) \subset dom H1 ->
     env_locs rho2 [set Γ] \subset dom H2 ->
     H1 ⊑ H1' ->
     H2 ⊑ H2' ->
-    FV_inv k j GII GI b rho1 H1 rho2 H2 c Scope Funs Γ FVs ->
-    FV_inv k j GII GI b rho1 H1' rho2 H2' c Scope Funs Γ FVs.
+    FV_inv k j GII GI b rho1 H1 rho2 H2 c Scope Γ FVs ->
+    FV_inv k j GII GI b rho1 H1' rho2 H2' c Scope Γ FVs.
   Proof.
     intros Hw1 Hw2 He1 He2 Hs1 Hs2.
     intros (x1 & x2 & Hget1 & Hget2 & Hall).
@@ -343,14 +318,14 @@ Module ClosureConversionCorrect (H : Heap).
     eapply In_Union_list. eapply in_map.
     eassumption.
   Qed.
-
+  
   (** [FV_inv] under rename extension  *)
   Lemma FV_inv_rename_ext (k j : nat) (GII : GIInv) (GI : GInv) (b b' : Inj)
         (rho1 : env) (H1 H2 : heap block) (rho2 : env) 
-        (c : cTag) (Scope Funs : Ensemble var) (Γ : var) (FVs : list var) :
-    FV_inv k j GII GI b rho1 H1 rho2 H2 c Scope Funs Γ FVs ->
-    f_eq_subdomain (reach' H1 (env_locs rho1 (FromList FVs \\ (Funs :|: Scope)))) b' b ->
-    FV_inv k j GII GI b' rho1 H1 rho2 H2 c Scope Funs Γ FVs.
+        (c : cTag) (Scope : Ensemble var) (Γ : var) (FVs : list var) :
+    FV_inv k j GII GI b rho1 H1 rho2 H2 c Scope Γ FVs ->
+    f_eq_subdomain (reach' H1 (env_locs rho1 (FromList FVs \\ Scope))) b' b ->
+    FV_inv k j GII GI b' rho1 H1 rho2 H2 c Scope Γ FVs.
   Proof.
     intros (x1 & x2 & Hget1 & Hget2 & Hall) Hfeq.
     repeat eexists; eauto.
@@ -361,321 +336,78 @@ Module ClosureConversionCorrect (H : Heap).
     eapply f_eq_subdomain_antimon; try eassumption.
     eapply reach'_set_monotonic.
     eapply get_In_env_locs; eauto.
-    constructor; eauto. rewrite Union_commut. eassumption.
+    constructor; eauto.
   Qed.
 
 
   (** [FV_inv] monotonic *)
   Lemma FV_inv_Scope_mon (k j : nat) (GII : GIInv) (GI : GInv) (b : Inj)
         (rho1 : env) (H1 H2 : heap block) (rho2 : env) 
-        (c : cTag) (Scope Scope' Funs : Ensemble var) (Γ : var) (FVs : list var) :
-    FV_inv k j GII GI b rho1 H1 rho2 H2 c Scope Funs Γ FVs ->
+        (c : cTag) (Scope Scope' : Ensemble var) (Γ : var) (FVs : list var) :
+    FV_inv k j GII GI b rho1 H1 rho2 H2 c Scope Γ FVs ->
     Scope \subset Scope' -> 
-    FV_inv k j GII GI b rho1 H1 rho2 H2 c Scope' Funs Γ FVs.
-  Proof.
-    intros (x1 & x2 & Hget1 & Hget2 & Hall) Hfeq.
-    repeat eexists; eauto. eapply Forall2_P_monotonic. eassumption.
-    now eauto with Ensembles_DB. 
-  Qed.
-
-  Lemma FV_inv_Funs_mon (k j : nat) (GII : GIInv) (GI : GInv) (b : Inj)
-        (rho1 : env) (H1 H2 : heap block) (rho2 : env) 
-        (c : cTag) (Scope Funs Funs' : Ensemble var) (Γ : var) (FVs : list var) :
-    FV_inv k j GII GI b rho1 H1 rho2 H2 c Scope Funs Γ FVs ->
-    Funs \subset Funs' -> 
-    FV_inv k j GII GI b rho1 H1 rho2 H2 c Scope Funs' Γ FVs.
+    FV_inv k j GII GI b rho1 H1 rho2 H2 c Scope' Γ FVs.
   Proof.
     intros (x1 & x2 & Hget1 & Hget2 & Hall) Hfeq.
     repeat eexists; eauto. eapply Forall2_P_monotonic. eassumption.
     now eauto with Ensembles_DB. 
   Qed.
   
-  (** * Lemmas about [Fun_inv] *)
-
-  Lemma Fun_inv_image_post (k j : nat) (GII : GIInv) (GI : GInv) (b : Inj)
-             (rho1 : env) (H1 : heap block) (rho2 : env) (H2 : heap block)
-             (Scope Funs : Ensemble var) :
-    Fun_inv k j GII GI b rho1 H1 rho2 H2 Scope Funs ->
-    image b ((post H1 ^ j) (env_locs rho1 (Funs \\ Scope))) <-->
-          (post H2 ^ j) (env_locs rho2 (Funs \\ Scope)).
-  Proof.
-    intros Hfun. split.
-    - intros l [l' [Hin Heq]]. subst.
-      edestruct post_n_exists_Singleton as [l'' [Hpost' Hin']]; eauto.
-      edestruct Hpost' as [f [Hinf Hgetf]]. inv Hinf.
-      edestruct Hfun as (lf1 & lf2 & Hget1 & Hget2 & Hrel); eauto.
-      rewrite Hget1 in Hgetf.
-      eapply cc_approx_val_image_eq in Hrel.
-      eapply post_n_set_monotonic.
-      eapply env_locs_monotonic.
-      eapply Singleton_Included. constructor; eauto.
-      eapply post_n_set_monotonic. eapply env_locs_Singleton; eauto.
-      eapply Hrel. eexists; split;  eauto.
-      eapply post_n_set_monotonic; eauto. eapply Singleton_Included. eassumption.
-    - intros l Hpost.
-      edestruct post_n_exists_Singleton as [l'' [Hpost' Hin']]; eauto.
-      edestruct Hpost' as [f' [Hin Hgetf]]; subst.
-      inv Hin.
-      edestruct Hfun as (lf1 & lf2 & Hget1 & Hget2 & Hrel); eauto.
-       eapply cc_approx_val_image_eq in Hrel.
-      rewrite Hget2 in Hgetf. destruct lf2; inv Hgetf. eapply Hrel in Hin'.
-      eapply image_monotonic; eauto.
-      eapply post_n_set_monotonic. eexists; split; eauto. constructor; eauto.
-      rewrite Hget1; eauto.
-  Qed.
   
-  Lemma Fun_inv_j_monotonic (k j' j : nat) (GII : GIInv) (GI : GInv) (b : Inj)
-        (rho1 : env) (H1 : heap block) (rho2 : env) (H2 : heap block)
-        (Scope Funs : Ensemble var) :
-    Fun_inv k j GII GI b rho1 H1 rho2 H2 Scope Funs  ->
-    j' <= j ->
-    Fun_inv k j' GII GI b rho1 H1 rho2 H2 Scope Funs .
-  Proof.
-    intros Hfv Hlt f Hin' Hin''.
-    edestruct Hfv as (lf1 & lf2 & Hget1 & Hget2 & Hrel); eauto.
-    repeat eexists; eauto.
-    eapply cc_approx_val_j_monotonic; eauto.
-  Qed.
-  
-  Lemma Fun_inv_monotonic (k k' j : nat) (GII : GIInv) (GI : GInv) (b : Inj)
-        (rho1 : env) (H1 : heap block) (rho2 : env) (H2 : heap block)
-        (Scope Funs : Ensemble var) :
-    Fun_inv k j GII GI b rho1 H1 rho2 H2 Scope Funs ->
-    k' <= k ->
-    Fun_inv k' j GII GI b rho1 H1 rho2 H2 Scope Funs.
-  Proof.
-    intros Hfv Hlt f Hin' Hin''.
-    edestruct Hfv as (lf1 & lf2 & Hget1 & Hget2 & Hrel); eauto.
-    repeat eexists; eauto.
-    eapply cc_approx_val_monotonic; eauto.
-  Qed.
-
-  Lemma Fun_inv_set_not_in_Funs_l (k  j : nat) (GII : GIInv) (GI : GInv) (b : Inj)
-        (rho1 : env) (H1 : heap block) (rho2 : env) (H2 : heap block)
-        (Scope Funs : Ensemble var) x v :
-    Fun_inv k j GII GI b rho1 H1 rho2 H2 Scope Funs  ->
-    ~ x \in (Funs \\ Scope) ->
-    Fun_inv k j GII GI b (M.set x v rho1) H1 rho2 H2 Scope Funs.
-  Proof.
-    intros Hfv Hlt f Hnin Hin.
-    edestruct Hfv as (lf1 & lf2 & Hget1 & Hget2 & Hrel); eauto.
-    repeat eexists; eauto.
-    rewrite M.gso; eauto. intros Hc; inv Hc; eauto.
-    eapply Hlt; constructor; eauto.
-  Qed.
-  
-  Lemma Fun_inv_set_not_in_Funs_r (k  j : nat) (GII : GIInv) (GI : GInv) (b : Inj)
-        (rho1 : env) (H1 : heap block) (rho2 : env) (H2 : heap block)
-        (Scope Funs : Ensemble var) x v :
-    Fun_inv k j GII GI b rho1 H1 rho2 H2 Scope Funs ->
-    ~ x \in (Funs \\ Scope) ->
-    Fun_inv k j GII GI b rho1 H1 (M.set x v rho2) H2 Scope Funs.
-  Proof.
-    intros Hfv Hlt f Hnin Hin.
-    edestruct Hfv as (lf1 & lf2 & Hget1 & Hget2 & Hrel); eauto.
-    repeat eexists; eauto.
-    rewrite M.gso; eauto. intros Hc; inv Hc; eauto.
-    eapply Hlt. constructor; eauto.
-  Qed.
-
-  Lemma Fun_inv_set_not_in_Funs (k  j : nat) (GII : GIInv) (GI : GInv) (b : Inj)
-        (rho1 : env) (H1 : heap block) (rho2 : env) (H2 : heap block)
-        (Scope Funs : Ensemble var) x y v v' :
-    Fun_inv k j GII GI b rho1 H1 rho2 H2 Scope Funs  ->
-    ~ x \in (Funs \\ Scope) ->
-    ~ y \in (Funs \\ Scope) ->
-    Fun_inv k j GII GI b (M.set x v rho1) H1 (M.set y v' rho2) H2 Scope Funs.
-  Proof.
-    intros Hfv Hnin Hnin'.
-    eapply Fun_inv_set_not_in_Funs_r; eauto.
-    eapply Fun_inv_set_not_in_Funs_l; eauto.
-  Qed.
-  
-  Lemma Fun_inv_image_reach (k : nat) (GII : GIInv) (GI : GInv) (b : Inj)
-             (rho1 : env) (H1 : heap block) (rho2 : env) (H2 : heap block)
-             (Scope Funs : Ensemble var) :
-    (forall j, Fun_inv k j GII GI b rho1 H1 rho2 H2 Scope Funs) ->
-    image b (reach' H1 (env_locs rho1 (Funs \\ Scope))) <-->
-    reach' H2 (env_locs rho2 (Funs \\ Scope)).
-  Proof.
-    intros Hfv. split.
-    - intros l' [l [[m [Hm Hr]] Hin]].
-      eexists m. split; eauto. eapply Fun_inv_image_post. eauto.
-      eexists; split; eauto.
-    - intros l' [m [Hm Hr]].
-      eapply Fun_inv_j_monotonic in Hfv; eauto.
-      eapply Fun_inv_image_post in Hr; eauto.
-      destruct Hr as [l [Heql Hin]]. eexists; split; eauto.
-      eexists; split; eauto.
-  Qed.
-  
-  Lemma Fun_inv_image_reach_n
-        (k j : nat) (GII : GIInv) (GI : GInv) (b : Inj)
-        (rho1 : env) (H1 : heap block) (rho2 : env) (H2 : heap block)
-        (Scope Funs : Ensemble var) :
-    Fun_inv k j GII GI b rho1 H1 rho2 H2 Scope Funs ->
-    image b (reach_n H1 j (env_locs rho1 (Funs \\ Scope))) <-->
-    (reach_n H2 j) (env_locs rho2 (Funs \\ Scope)).
-  Proof.
-    intros Hfv. split.
-    - intros l' [l [[m [Hm Hr]] Hin]].
-      eapply Fun_inv_j_monotonic in Hfv; eauto.
-      eexists m. split; eauto. eapply Fun_inv_image_post. eassumption.
-      eexists; split; eauto.
-    - intros l' [m [Hm Hr]].
-      eapply Fun_inv_j_monotonic in Hfv; eauto.
-      eapply Fun_inv_image_post in Hr; eauto.
-      destruct Hr as [l [Heql Hin]]. eexists; split; eauto.
-      eexists; split; eauto.
-  Qed.
-  
-  Lemma Fun_inv_weak_in_Fun_inv k j P1 P2 rho1 H1 rho2 H2 β Scope Funs :
-    Fun_inv k j P1 P2 β rho1 H1 rho2 H2 Scope Funs ->
-    Fun_inv_weak rho1 H1 rho2 H2 Scope Funs.
-  Proof.
-    now firstorder. 
-  Qed.
-
-  (** [Fun_inv] is heap monotonic  *)
-  Lemma Fun_inv_heap_mon (k  j : nat) (GII : GIInv) (GI : GInv) (b : Inj)
-        (rho1 : env) (H1 H1' : heap block) (rho2 : env) (H2 H2' : heap block)
-        (Scope Funs : Ensemble var) :
-    well_formed (reach' H1 (env_locs rho1 (Funs \\ Scope))) H1 ->
-    well_formed (reach' H2 (env_locs rho2 (Funs \\ Scope))) H2 ->
-    env_locs rho1 (Funs \\ Scope) \subset dom H1 ->
-    env_locs rho2 (Funs \\ Scope) \subset dom H2 ->
-    H1 ⊑ H1' ->
-    H2 ⊑ H2' ->
-    Fun_inv k j GII GI b rho1 H1 rho2 H2 Scope Funs ->
-    Fun_inv k j GII GI b rho1 H1' rho2 H2' Scope Funs.
-  Proof.
-    intros Hw1 Hw2 He1 He2 Hs1 Hs2 Hfv x Hnin Hin.
-    edestruct Hfv as (lf1 & lf2 & Hget1 & Hget2 & Hrel); eauto.
-    repeat eexists; eauto.
-    eapply cc_approx_val_heap_monotonic; try eassumption.
-    eapply well_formed_antimon; [| eassumption ].
-    eapply reach'_set_monotonic. eapply get_In_env_locs; eauto.
-    now constructor; eauto.
-    eapply well_formed_antimon; [| eassumption ].
-    eapply reach'_set_monotonic. eapply get_In_env_locs; eauto.
-    constructor; eauto.
-    eapply Included_trans; [| eassumption ]. eapply get_In_env_locs; eauto.
-    now constructor; eauto.
-    eapply Included_trans; [| eassumption ]. eapply get_In_env_locs; eauto.
-    now constructor; eauto.
-  Qed.
-  
-
-  (** [Fun_inv] under renaming extension  *)
-  Lemma Fun_inv_rename_ext (k  j : nat) (GII : GIInv) (GI : GInv) (b b' : Inj)
-        (rho1 : env) (H1  : heap block) (rho2 : env) (H2 : heap block)
-        (Scope Funs : Ensemble var) :
-    Fun_inv k j GII GI b rho1 H1 rho2 H2 Scope Funs  ->
-    f_eq_subdomain (reach' H1 (env_locs rho1 (Funs \\ Scope))) b' b ->
-    Fun_inv k j GII GI b' rho1 H1 rho2 H2 Scope Funs.
-  Proof.
-    intros Hfv Hfeq f Hnin Hin.
-    edestruct Hfv as (lf1 & lf2 & Hget1 & Hget2 & Hrel); eauto.
-    repeat eexists; eauto.
-    eapply cc_approx_val_rename_ext; try eassumption.
-    eapply f_eq_subdomain_antimon; [| eassumption ].
-    eapply reach'_set_monotonic.
-    eapply get_In_env_locs; eauto. constructor; eauto.
-  Qed.
-  
-  (** [Fun_inv] monotonic *)
-  Lemma Fun_inv_Scope_mon (k j : nat) (GII : GIInv) (GI : GInv) (b : Inj)
-        (rho1 : env) (H1 H2 : heap block) (rho2 : env) 
-        (Scope Scope' Funs : Ensemble var) :
-    Fun_inv k j GII GI b rho1 H1 rho2 H2 Scope Funs ->
-    Scope \subset Scope' -> 
-    Fun_inv k j GII GI b rho1 H1 rho2 H2 Scope' Funs.
-  Proof.
-    intros Hf Hsub. intros x Hin Hin'. eapply Hf; eauto.
-  Qed.
-  
-  
-  (* Lemma ctx_to_heap_env_size_heap C rho1 rho2 H1 H2 c : *)
-  (*   ctx_to_heap_env C H1 rho1 H2 rho2 c -> *)
-  (*   size_heap H2 = size_heap H1 + cost_alloc_ctx C. *)
-  (* Proof. *)
-  (*   intros Hctx; induction Hctx; eauto. *)
-  (*   simpl. rewrite IHHctx. *)
-  (*   unfold size_heap. *)
-  (*   erewrite (HL.size_with_measure_alloc _ _ _ H H'); *)
-  (*     [| reflexivity | eassumption ]. *)
-  (*   erewrite getlist_length_eq; [| eassumption ]. *)
-  (*   simpl. omega. *)
-  (* Qed. *)
-
-  (** Process the evaluation context of the right expression *)
-
   (** * Lemmas about [project_var] and [project_vars] *)
   
     
-  Lemma project_var_ctx_to_heap_env Scope Funs c Γ FVs x x' C S S' v1 rho1 rho2 H1 H2:
-    project_var Scope Funs c Γ FVs S x x' C S' ->
-    Fun_inv_weak rho1 H1 rho2 H2 Scope Funs  ->
-    FV_inv_weak rho1 rho2 H2 c Scope Funs Γ FVs ->
+  Lemma project_var_ctx_to_heap_env Scope c Γ FVs x x' C S S' v1 rho1 rho2 H2:
+    project_var Scope c Γ FVs S x x' C S' ->
+    FV_inv_weak rho1 rho2 H2 c Scope Γ FVs ->
     M.get x rho1 = Some v1 ->
     exists H2' rho2' s, ctx_to_heap_env_CC C H2 rho2 H2' rho2' s.
   Proof.
-    intros Hproj HFun HFV Hget. inv Hproj.
+    intros Hproj HFV Hget. inv Hproj.
     - repeat eexists; econstructor; eauto.
-    - edestruct HFun as
-          (vf1 & vf4 & Hget1 & Hget2) ; eauto.
-      repeat eexists; constructor; eauto.
     - edestruct HFV as (v & vs  & Hget1 & Hget2 & Hall).
-      edestruct Forall2_P_nthN as [v2 [Hnth Hr]]; eauto. 
-      intros Hc; inv Hc; eauto.
+      edestruct Forall2_P_nthN as [v2 [Hnth Hr]]; eauto.
       repeat eexists. econstructor; eauto.
       constructor.
   Qed.
   
-  Lemma project_vars_ctx_to_heap_env Scope Funs c Γ FVs xs xs' C S S' vs1 rho1 H1 rho2 H2:
-    Disjoint _ S (FV_cc Scope Funs Γ) ->
+  Lemma project_vars_ctx_to_heap_env Scope c Γ FVs xs xs' C S S' vs1 rho1 rho2 H2:
+    Disjoint _ S (FV_cc Scope Γ) ->
     
-    project_vars Scope Funs c Γ FVs S xs xs' C S' ->
-    Fun_inv_weak rho1 H1 rho2 H2 Scope Funs ->
-    FV_inv_weak rho1 rho2 H2 c Scope Funs Γ FVs ->
+    project_vars Scope c Γ FVs S xs xs' C S' ->
+    FV_inv_weak rho1 rho2 H2 c Scope Γ FVs ->
     getlist xs rho1 = Some vs1 ->
     exists H2' rho2' s, ctx_to_heap_env_CC C H2 rho2 H2' rho2' s.
   Proof.
-    intros HD Hvars HFun HFV.
-    revert Scope Funs Γ FVs xs' C S S' vs1
-           rho1 rho2 H2 HD  Hvars HFun HFV.
+    intros HD Hvars HFV.
+    revert Scope Γ FVs xs' C S S' vs1
+           rho1 rho2 H2 HD  Hvars HFV.
     induction xs;
-      intros Scope Funs Γ FVs xs' C S S' vs1
-             rho1 rho2 H2 HD Hvars HFun HFV Hgetlist.
+      intros Scope Γ FVs xs' C S S' vs1
+             rho1 rho2 H2 HD Hvars HFV Hgetlist.
     - inv Hvars. repeat eexists; econstructor; eauto.
     - inv Hvars. simpl in Hgetlist.
       destruct (M.get a rho1) eqn:Hgeta1; try discriminate.
       destruct (getlist xs rho1) eqn:Hgetlist1; try discriminate.
       edestruct project_var_ctx_to_heap_env with (rho1 := rho1) as [H2' [rho2' [s Hctx1]]]; eauto.
       inv Hgetlist.
-      edestruct IHxs with (H2 := H2') (rho2 := rho2') as [H2'' [rho2'' [s' Hctx2]]]; [| eassumption | | | eassumption | ].
+      edestruct IHxs with (H2 := H2') (rho2 := rho2') as [H2'' [rho2'' [s' Hctx2]]]; [| eassumption | | eassumption | ].
       + eapply Disjoint_Included_l; [| eassumption ].
         eapply project_var_free_set_Included. eassumption.
-      + intros f Hin Hnin.
-        edestruct HFun as (vf1 & vf2 & Hgetf1 & Hgetf2); try eassumption.
-        repeat eexists; eauto.
-        erewrite <- project_var_get; try eassumption.
-        intros Hin'. eapply HD. constructor. now eauto.
-        left. right.  constructor; eauto.
       + edestruct HFV as [v' [vs [Hget [Hget1 Hall]]]]; eauto.
         repeat eexists; eauto.
         * erewrite <- project_var_get; try eassumption.
           intros Hin'. eapply HD. constructor. now eauto.
           right. reflexivity.
-        * erewrite <- (project_var_heap _ _ _ _ _ _ _ _ _ _ _ _ _ _ _ H9). eassumption.
+        * erewrite <- (project_var_heap _ _ _ _ _ _ _ _ _ _ _ _ _ _ H7). eassumption.
           eassumption.
       + exists H2'', rho2'', (s + s'). eapply ctx_to_heap_env_CC_comp_ctx_f_r; eassumption.
   Qed.
   
 
   Lemma project_var_preserves_cc_approx GII GI k j H1 rho1 H2 rho2 H2' rho2' b
-        Scope Funs c Γ FVs x x' C S S' m y y' :
-    project_var Scope Funs c Γ FVs S x x' C S' ->
+        Scope c Γ FVs x x' C S S' m y y' :
+    project_var Scope c Γ FVs S x x' C S' ->
     cc_approx_var_env k j GII GI b H1 rho1 H2 rho2 y y' ->
     ctx_to_heap_env_CC C H2 rho2 H2' rho2' m ->
     ~ y' \in S ->
@@ -683,13 +415,13 @@ Module ClosureConversionCorrect (H : Heap).
   Proof.     
     intros Hproj Hcc Hctx Hnin.
     destruct Hproj; inv Hctx; eauto.
-    - inv H19. eapply cc_approx_var_env_set_neq_r; eauto.
+    - inv H18. eapply cc_approx_var_env_set_neq_r; eauto.
       intros Hc; subst; eauto.
   Qed.
   
   Lemma project_vars_preserves_cc_approx GII GI k j H1 rho1 H2 rho2 H2' rho2' b
-        Scope Funs c Γ FVs xs xs' C S S' m y y' :
-    project_vars Scope Funs c Γ FVs S xs xs' C S' ->
+        Scope c Γ FVs xs xs' C S S' m y y' :
+    project_vars Scope c Γ FVs S xs xs' C S' ->
     cc_approx_var_env k j GII GI b H1 rho1 H2 rho2 y y' ->
     ctx_to_heap_env_CC C H2 rho2 H2' rho2' m ->
     ~ y' \in S ->
@@ -708,48 +440,34 @@ Module ClosureConversionCorrect (H : Heap).
 
   (** Correctness of [project_var] *)
   Lemma project_var_correct GII GI k  H1 rho1 H2 rho2 H2' rho2' b
-        Scope Funs c Γ FVs x x' C S S' m :
-    project_var Scope Funs c Γ FVs S x x' C S' ->
+        Scope c Γ FVs x x' C S S' m :
+    project_var Scope c Γ FVs S x x' C S' ->
     
     (forall j, (H1, rho1) ⋞ ^ (Scope; k; j; GII; GI; b) (H2, rho2)) ->
-    (forall j, Fun_inv k j GII GI b rho1 H1 rho2 H2 Scope Funs) ->
-    (forall j, FV_inv k j GII GI b rho1 H1 rho2 H2 c Scope Funs Γ FVs) ->
+    (forall j, FV_inv k j GII GI b rho1 H1 rho2 H2 c Scope Γ FVs) ->
 
     ctx_to_heap_env_CC C H2 rho2 H2' rho2' m ->
     
     binding_in_map Scope rho1 ->
-    Disjoint _ S (FV_cc Scope Funs Γ) ->
+    Disjoint _ S (FV_cc Scope Γ) ->
 
     ~ In _ S' x' /\
     (forall j, (H1, rho1) ⋞ ^ (Scope; k; j; GII; GI; b) (H2', rho2'))  /\
-    (forall j, Fun_inv k j GII GI b rho1 H1 rho2' H2' Scope Funs) /\
-    (forall j, FV_inv k j GII GI b rho1 H1 rho2' H2' c Scope Funs Γ FVs) /\
+    (forall j, FV_inv k j GII GI b rho1 H1 rho2' H2' c Scope Γ FVs) /\
     (forall j, cc_approx_var_env k j GII GI b H1 rho1 H2' rho2' x x').
 
   Proof with (now eauto with Ensembles_DB).
-    intros Hproj Hcc Hfun Henv Hctx Hbin Hd.
+    intros Hproj Hcc Henv Hctx Hbin Hd.
     inv Hproj.
     - inv Hctx. split. intros Hc. eapply Hd; eauto. constructor; eauto. left; eauto.
-      split; [| split; [| split ]]; eauto.
+      split; [| split ]; eauto.
       intros j; eapply Hcc. eassumption.
-    - inv Hctx.
-      split; [| split; [| split; [| split ]]]. repeat split.
-      + intros Hc. eapply Hd. constructor; eauto.
-        left. right. constructor; eauto.
-      + intros j. eapply Hcc; eauto.
-      + eassumption.
-      + eassumption.
-      + intros j. edestruct (Hfun j) as (vf1 & vf2 & Hget1 & Hget2 & Hcc'); eauto.
-        intros v1 Hget1'. repeat subst_exp. eexists; split; eauto.
-    - inv Hctx. inv H19.
-      split; [| split; [| split; [| split ]]]. repeat split.
+    - inv Hctx. inv H18.
+      split; [| split; [| split ]]. repeat split.
       + intros Hc. inv Hc. eauto.
       + intros j. eapply cc_approx_env_P_set_not_in_P_r. now eauto.
         intros Hc. eapply Hd; eauto. constructor; eauto.
         left; eauto.
-      + intros j. eapply Fun_inv_set_not_in_Funs_r; eauto.
-        intros Hc; eapply Hd. constructor; eauto.
-        constructor; eauto.
       + intros h. 
         edestruct Henv as (v1 & vs1 & Hget1 & Hget2 & Hall).
         repeat eexists; eauto. 
@@ -758,82 +476,58 @@ Module ClosureConversionCorrect (H : Heap).
       + intros j v' Hget.
         edestruct (Henv j) as (v1 & vs1 & Hget1 & Hget2 & Hall).
         eexists. rewrite M.gss. split. reflexivity.
-        edestruct (Forall2_P_nthN _ _ _ _ FVs _ N _ Hall H3) as (v2 & Hnth' & vs4 & Hget4 & Hrel).
-        intros Hc; inv Hc; eauto. repeat subst_exp. eassumption.
+        edestruct (Forall2_P_nthN _ _ _ _ FVs _ N _ Hall H0) as (v2 & Hnth' & vs4 & Hget4 & Hrel).
+        eassumption. repeat subst_exp. eassumption.
   Qed.
   
-  Lemma project_var_setminus_same  Scope Funs c Γ FVs x x' C S S' : 
-    project_var Scope Funs c Γ FVs S x x' C S' ->
-    project_var Scope (Funs \\ Scope) c Γ FVs S x x' C S'.
-  Proof. 
-    intros Hvar; destruct Hvar; try now constructor; eauto.
-    constructor; eauto. intros Hc; inv Hc; eauto.
-  Qed.
-
-  Lemma project_vars_setminus_same  Scope Funs c Γ FVs xs xs' C S S' : 
-    project_vars Scope Funs c Γ FVs S xs xs' C S' ->
-    project_vars Scope (Funs \\ Scope) c Γ FVs S xs xs' C S'.
-  Proof. 
-    intros Hvar; induction Hvar; try now constructor; eauto.
-    econstructor; eauto. eapply project_var_setminus_same. eassumption.
-  Qed.
-
   (** Correctness of [project_vars] *)
   Lemma project_vars_correct GII GI k  H1 rho1 H2 rho2 H2' rho2' b
-        Scope Funs c Γ FVs xs xs' C S S' m :
-    project_vars Scope Funs c Γ FVs S xs xs' C S' ->
+        Scope c Γ FVs xs xs' C S S' m :
+    project_vars Scope c Γ FVs S xs xs' C S' ->
     
     (forall j, (H1, rho1) ⋞ ^ (Scope; k; j; GII; GI; b) (H2, rho2)) ->
-    (forall j, Fun_inv k j GII GI b rho1 H1 rho2 H2 Scope Funs) ->
-    (forall j, FV_inv k j GII GI b rho1 H1 rho2 H2 c Scope Funs Γ FVs) ->
+    (forall j, FV_inv k j GII GI b rho1 H1 rho2 H2 c Scope Γ FVs) ->
 
     ctx_to_heap_env_CC C H2 rho2 H2' rho2' m ->
 
     binding_in_map Scope rho1 -> 
-    Disjoint _ S (FV_cc Scope Funs Γ) ->
+    Disjoint _ S (FV_cc Scope Γ) ->
 
     Disjoint _ (FromList xs') S' /\
     (forall j, (H1, rho1) ⋞ ^ (Scope; k; j; GII; GI; b) (H2', rho2'))  /\
-    (forall j, Fun_inv k j GII GI b rho1 H1 rho2' H2' Scope Funs) /\
-    (forall j, FV_inv k j GII GI b rho1 H1 rho2' H2' c Scope Funs Γ FVs) /\
+    (forall j, FV_inv k j GII GI b rho1 H1 rho2' H2' c Scope Γ FVs) /\
     (forall j, Forall2 (fun x x' => cc_approx_var_env k j GII GI b H1 rho1 H2' rho2' x x') xs xs').
   Proof with (now eauto with Ensembles_DB).
     intros Hvars. revert m H1 rho1 H2 rho2 H2' rho2'.
-    induction Hvars; intros m H1 rho1 H2 rho2 H2' rho2' Hcc Hfun Hfv Hctx Hb Hd. 
-    - inv Hctx. split; [| split; [| split ; [| split ]]]; eauto.
+    induction Hvars; intros m H1 rho1 H2 rho2 H2' rho2' Hcc Hfv Hctx Hb Hd. 
+    - inv Hctx. split; [| split; [| split ]]; eauto.
       rewrite FromList_nil...
     - rewrite FromList_cons in *. 
       edestruct ctx_to_heap_env_CC_comp_ctx_f_l as [rho3 [H3 [m1 [m2 [Hctx2 [Hctx3 Heq]]]]]].
       subst.
       eassumption. subst.
-      edestruct project_var_correct as (Hd' & Hcc' & Hfun' & Hfv' & Hall');
+      edestruct project_var_correct as (Hd' & Hcc' & Hfv' & Hall');
         try eassumption.
-      edestruct IHHvars as (Hd'' & Hcc'' & Hfun'' & Hfv'' & Hall'');
+      edestruct IHHvars as (Hd'' & Hcc'' & Hfv'' & Hall'');
       try eassumption.
       eapply Disjoint_Included_l; [| eassumption ].
       eapply project_var_free_set_Included. eassumption.
-      split; [| split; [| split ; [| split ]]]; eauto.
+      split; [| split; [| split ]]; eauto.
       * eapply Union_Disjoint_l. 
         eapply Disjoint_Included_r.
         eapply project_vars_free_set_Included. eassumption.
-        eapply Disjoint_Singleton_l.
-        eapply project_var_not_In_free_set'. eassumption.
+        eapply Disjoint_Singleton_l. eassumption.
         eapply Disjoint_Included_r; [| eassumption ].
         unfold FV_cc...
-        eapply Disjoint_sym. eapply project_vars_not_In_free_set'. eassumption.
-        eapply Disjoint_Included_l.
-        eapply project_var_free_set_Included. eassumption.
-        eapply Disjoint_Included_r; [| eassumption ].
-        unfold FV_cc...
-      * intros j. constructor; eauto .
+      * intros j. constructor; eauto.
         eapply project_vars_preserves_cc_approx; eauto.
   Qed.
 
   (** [project_var] preserves injectiveness *)
   Lemma project_var_same_set
-        Scope Funs c Γ FVs x x' C S S'  :
-    project_var Scope Funs c Γ FVs S x x' C S' ->
-    x |: (FV Scope Funs FVs) <--> FV Scope Funs FVs.
+        Scope c Γ FVs x x' C S S'  :
+    project_var Scope c Γ FVs S x x' C S' ->
+    x |: (FV Scope FVs) <--> FV Scope FVs.
   Proof with (now eauto with Ensembles_DB).
     intros Hvar. rewrite Union_Same_set. reflexivity.
     eapply Singleton_Included. eapply project_var_In_Union.
@@ -841,50 +535,43 @@ Module ClosureConversionCorrect (H : Heap).
   Qed.
 
   Lemma project_vars_same_set
-        Scope Funs c Γ FVs x x' C S S'  :
-    project_vars Scope Funs c Γ FVs S x x' C S' ->
-    (FromList x) :|: (FV Scope Funs FVs) <--> FV Scope Funs FVs.
+        Scope c Γ FVs x x' C S S'  :
+    project_vars Scope c Γ FVs S x x' C S' ->
+    (FromList x) :|: (FV Scope FVs) <--> FV Scope FVs.
   Proof with (now eauto with Ensembles_DB).
     intros Hvar. rewrite Union_Same_set. reflexivity.
     eapply project_vars_In_Union.
     eassumption.
   Qed.
 
-  Lemma image_FV GI GP k β H1 rho1 H2 rho2 Scope Funs FVs Γ c :
+  Lemma image_FV GI GP k β H1 rho1 H2 rho2 Scope `{Decidable _ Scope} FVs Γ c :
     (forall j, (H1, rho1) ⋞ ^ (Scope ; k ; j ; GI ; GP ; β) (H2, rho2)) ->
-    (forall j, Fun_inv k j GI GP β rho1 H1 rho2 H2 Scope Funs) ->
-    (forall j, FV_inv k j GI GP β rho1 H1 rho2 H2 c Scope Funs Γ FVs) ->
+    (forall j, FV_inv k j GI GP β rho1 H1 rho2 H2 c Scope Γ FVs) ->
     binding_in_map Scope rho1 ->
 
-    (image β (reach' H1 (env_locs rho1 (FV Scope Funs FVs)))) \subset
-    reach' H2 ((env_locs rho2 (Scope :|: (Funs \\ Scope))) :|: (post H2 (env_locs rho2 [set Γ]))).
+    (image β (reach' H1 (env_locs rho1 (FV Scope FVs)))) \subset
+    reach' H2 (env_locs rho2 Scope :|: (post H2 (env_locs rho2 [set Γ]))).
   Proof.
     intros. unfold FV, FV_cc.
     rewrite !env_locs_Union, !reach'_Union, !image_Union.
     rewrite cc_approx_env_image_reach; try eassumption. 
-    rewrite Fun_inv_image_reach; try eassumption.
     eapply Included_Union_compat. reflexivity.
     eapply FV_inv_image_reach; try eassumption.
   Qed.     
 
-  Lemma image_FV_eq GI GP k β H1 rho1 H2 rho2 Scope Funs FVs Γ c :
+  Lemma image_FV_eq GI GP k β H1 rho1 H2 rho2 Scope `{Decidable _ Scope} FVs Γ c :
     (forall j, (H1, rho1) ⋞ ^ (Scope ; k ; j ; GI ; GP ; β) (H2, rho2)) ->
-    (forall j, Fun_inv k j GI GP β rho1 H1 rho2 H2 Scope Funs) ->
-    (forall j, FV_inv k j GI GP β rho1 H1 rho2 H2 c Scope Funs Γ FVs) ->
+    (forall j, FV_inv k j GI GP β rho1 H1 rho2 H2 c Scope Γ FVs) ->
     binding_in_map Scope rho1 ->
-    Disjoint var (FromList FVs) (Scope :|: Funs) ->
-    (image β (reach' H1 (env_locs rho1 (FV Scope Funs FVs)))) <-->
-    reach' H2 ((env_locs rho2 (Scope :|: (Funs \\ Scope))) :|: (post H2 (env_locs rho2 [set Γ]))).
+    Disjoint var (FromList FVs) Scope ->
+    (image β (reach' H1 (env_locs rho1 (FV Scope FVs)))) <-->
+    reach' H2 (env_locs rho2 Scope :|: (post H2 (env_locs rho2 [set Γ]))).
   Proof.
     intros. unfold FV, FV_cc.
     rewrite !env_locs_Union, !reach'_Union, !image_Union.
     rewrite cc_approx_env_image_reach; try eassumption. 
-    rewrite Fun_inv_image_reach; try eassumption.
-    assert (Hd' := H5). eapply Setminus_Disjoint in H5.
     eapply Same_set_Union_compat. reflexivity.
-    eapply Same_set_trans. eapply image_Proper_Same_set. (* ?????? *)
-    reflexivity. eapply Proper_reach'. reflexivity.
-    eapply Proper_env_locs. reflexivity. eassumption.
+    rewrite Setminus_Disjoint; [| eassumption ].
     rewrite FV_inv_image_reach_eq; try eassumption. reflexivity.
   Qed.
 
@@ -961,8 +648,8 @@ Module ClosureConversionCorrect (H : Heap).
     eapply make_closures_env_locs_well_formed.
   Qed.
 
-  (* Definition pre_Fun_inv k j IP P b rho1 H1 rho2 H2 Funs Γ := *)
-  (*   forall f, f \in Funs -> *)
+  (* Definition pre_Fun_inv k j IP P b rho1 H1 rho2 H2 Γ := *)
+  (*   forall f, f \in -> *)
   (*        exists l1 v1 v2 b1, *)
   (*          M.get f rho1 = Some (Loc l1) /\ *)
   (*          get l1 H1 = Some b1 /\ *)
@@ -970,18 +657,19 @@ Module ClosureConversionCorrect (H : Heap).
   (*          M.get Γ rho2 = Some v2 /\ *)
   (*          cc_approx_block k j IP P b b1 H1 (Constr Size.Util.clo_tag [v1; v2]) H2.      *)
 
+  (* 
 
   Lemma make_closures_Fun_inv k j GI GP b C rho1 H1 rho2 H1' rho1' H2 rho2'
-        H2' Scope Funs B1 B2 B1' B2'
+        H2' Scope B1 B2 B1' B2'
         Γ fvs B' fvs' m l1 l2 :
 
    (* well_formed (reach' H1 (env_locs rho1 ())) H1 -> *)
    (* env_locs rho1 (Scope :|: (name_in_fundefs B1)) \subset dom H1  -> *)
-   (* well_formed (reach' H2 (env_locs rho2 (fvs :|: Funs :|: [set Γ]))) H2 -> *)
-   (* env_locs rho2 (fvs :|: Funs :|: [set Γ]) \subset dom H2  -> *)
-   (* injective_subdomain (reach' H1 (env_locs rho1 (FV Scope Funs FVs))) b -> *)
+   (* well_formed (reach' H2 (env_locs rho2 (fvs :|: :|: [set Γ]))) H2 -> *)
+   (* env_locs rho2 (fvs :|: :|: [set Γ]) \subset dom H2  -> *)
+   (* injective_subdomain (reach' H1 (env_locs rho1 (FV Scope FVs))) b -> *)
 
-   Closure_conversion_fundefs B' Size.Util.clo_tag fvs' B1 B2 ->
+   Closure_conversion_fundefs  Size.Util.clo_tag B' fvs' B1 B2 ->
    make_closures Size.Util.clo_tag B1 fvs Γ C ->
    
    def_closures B1 B1' rho1 l1 = (H1', rho2') ->
@@ -1243,51 +931,45 @@ Module ClosureConversionCorrect (H : Heap).
   (*     * intros j. constructor; eauto . *)
   (*       eapply project_vars_preserves_cc_approx; eauto. *)
   (* Qed. *)
-
+*)
   
   (** Correctness of [Closure_conversion] *)
   Lemma Closure_conversion_correct (k : nat) (H1 H2 : heap block)
         (rho1 rho2 : env) (e1 e2 : exp) (C : exp_ctx)
-        (Scope Funs : Ensemble var) `{ToMSet Funs} (FVs : list var)
+        (Scope Funs : Ensemble var) `{HD: Decidable _ Scope} `{ToMSet Funs} (FVs : list var)
         (β : Inj) (c : cTag) (Γ : var) :
     (* [Scope] invariant *)
     (forall j, (H1, rho1) ⋞ ^ (Scope ; k ; j ; PreG Funs; (fun i => Post 0) ; β) (H2, rho2)) ->
-    (* [Fun] invariant *)
-    (forall j, Fun_inv k j (PreG Funs) (fun i => Post 0) β rho1 H1 rho2 H2 Scope Funs) ->
     (* Free variables invariant *)
-    (forall j, FV_inv k j (PreG Funs) (fun i => Post 0) β rho1 H1 rho2 H2 c Scope Funs Γ FVs) ->
+    (forall j, FV_inv k j (PreG Funs) (fun i => Post 0) β rho1 H1 rho2 H2 c Scope Γ FVs) ->
     (* location renaming is injective *)
     (* only needed to prove the lower bound *)
-    injective_subdomain (reach' H1 (env_locs rho1 (FV Scope Funs FVs))) β ->
+    injective_subdomain (reach' H1 (env_locs rho1 (FV Scope FVs))) β ->
     
     (* well-formedness *)
-    well_formed (reach' H1 (env_locs rho1 (FV Scope Funs FVs))) H1 ->
-    (env_locs rho1 (FV Scope Funs FVs)) \subset dom H1 ->
-    well_formed (reach' H2 (env_locs rho2 (FV_cc Scope Funs Γ))) H2 ->
-    (env_locs rho2 (FV_cc Scope Funs Γ)) \subset dom H2 ->
-
+    well_formed (reach' H1 (env_locs rho1 (FV Scope FVs))) H1 ->
+    (env_locs rho1 (FV Scope FVs)) \subset dom H1 ->
+    well_formed (reach' H2 (env_locs rho2 (FV_cc Scope Γ))) H2 ->
+    (env_locs rho2 (FV_cc Scope Γ)) \subset dom H2 ->
     
     (* [Γ] (the current environment parameter) is not bound in e *)
     ~ In _ (bound_var e1) Γ ->
     (* The free variables of e are defined in the environment *)
-    binding_in_map (FV Scope Funs FVs) rho1 ->
+    binding_in_map (FV Scope FVs) rho1 ->
     (* The blocks of functions have unique function names *)
     fundefs_names_unique e1 ->
-    (* function renaming codomain is not shadowed by other vars *)
-    Disjoint _ (Funs \\ Scope) (bound_var e1) ->
-
     
     (* [e'] is the closure conversion of [e] *)
-    Closure_conversion Size.Util.clo_tag Scope Funs c Γ FVs e1 e2 C ->
+    Closure_conversion Size.Util.clo_tag Scope c Γ FVs e1 e2 C ->
     
     (forall j, (e1, rho1, H1) ⪯ ^ (k ; j ; Pre ; PreG Funs ; Post 0 ; fun i => Post 0) (C |[ e2 ]|, rho2, H2)).
   Proof with now eauto with Ensembles_DB.
-    revert H1 H2 rho1 rho2 e1 e2 C Scope Funs H FVs β c Γ.
+    revert H1 H2 rho1 rho2 e1 e2 C Scope HD Funs H FVs β c Γ.
     induction k as [k IHk] using lt_wf_rec1.
-    intros H1 H2 rho1 rho2 e1 e2 C Scope Funs HMSet FVs β c Γ
-           Henv Hfun HFVs Hinjb Hwf1 Hlocs1 Hwf2 Hlocs2 Hnin Hbind Hun Hd Hcc.
-    assert (Hfv := Closure_conversion_pre_occurs_free_Included _ _ _ _ _ _ _ _ Hcc).
-    assert (Hfv' := Closure_conversion_occurs_free_Included _ _ _ _ _ _ _ _ Hcc Hun).
+    intros H1 H2 rho1 rho2 e1 e2 C Scope HD Funs HMSet FVs β c Γ
+           Henv HFVs Hinjb Hwf1 Hlocs1 Hwf2 Hlocs2 Hnin Hbind Hun Hcc.
+    assert (Hfv := Closure_conversion_pre_occurs_free_Included _ _ _ _ _ _ _ Hcc).
+    assert (Hfv' := Closure_conversion_occurs_free_Included _ _ _ _ _ _ _ Hcc Hun).
     induction e1 using exp_ind'; try clear IHe1.
     - (* case Econstr *)
       inv Hcc.
@@ -1296,7 +978,6 @@ Module ClosureConversionCorrect (H : Heap).
       eapply project_vars_In_Union. eassumption.
       
       edestruct project_vars_ctx_to_heap_env as [H2' [rho2' [m Hct]]]; try eassumption.
-      specialize (Hfun 0); eapply Fun_inv_weak_in_Fun_inv; eassumption.
       specialize (HFVs 0); eapply FV_inv_weak_in_FV_inv; eassumption.
       
       intros j.
@@ -1324,7 +1005,7 @@ Module ClosureConversionCorrect (H : Heap).
       eapply project_vars_env_locs' in Hlocs2; try eassumption;
       [| eapply Disjoint_Included_r; try eassumption; unfold FV_cc; now eauto with Ensembles_DB ].
       
-      edestruct project_vars_correct as (Hd' & Henv' & Hfun' & HFVs' & Hvars);
+      edestruct project_vars_correct as (Hd' & Henv' & HFVs' & Hvars);
         try eassumption.
       eapply binding_in_map_antimon; [| eassumption ]...
       
@@ -1352,7 +1033,7 @@ Module ClosureConversionCorrect (H : Heap).
       + (* Inductive case *)  
         intros vs1 vs2 l1 l2 H1' H2'' Hleq Ha1 Ha2 Hr1 Hr2 Hall j1.
         (* monotonicity of the local invariant *) 
-        assert (Hfeq : f_eq_subdomain (reach' H1 (env_locs rho1 (FV Scope Funs FVs))) β (β {l1 ~> l2})).
+        assert (Hfeq : f_eq_subdomain (reach' H1 (env_locs rho1 (FV Scope FVs))) β (β {l1 ~> l2})).
         { eapply f_eq_subdomain_extend_not_In_S_r; [| reflexivity ].
           intros Hc. eapply reachable_in_dom in Hc.
           edestruct Hc as [vc Hgetc]. erewrite alloc_fresh in Hgetc; eauto. congruence.
@@ -1361,6 +1042,7 @@ Module ClosureConversionCorrect (H : Heap).
         { eapply IHk;
           [ | | | | | | | | | | | | eassumption ].
           * simpl in *. omega.
+          * now eauto with typeclass_instances.
           * { intros j2.  
               eapply cc_approx_env_set_alloc_Constr with (b := β {l1 ~> l2});
                 try eassumption.
@@ -1404,7 +1086,7 @@ Module ClosureConversionCorrect (H : Heap).
               - rewrite extend_gss. reflexivity.
               - intros j3 Hlt3. eapply Forall2_monotonic_strong; [| now eapply Hall ].
                 intros x1 x2 Hin1 Hin2 Hrel. eapply cc_approx_val_rename_ext. now eapply Hrel.
-                assert (Hincl : val_loc x1 \subset env_locs rho1 (FV Scope Funs FVs)).
+                assert (Hincl : val_loc x1 \subset env_locs rho1 (FV Scope FVs)).
                 { eapply Included_trans; [| now eapply env_locs_monotonic; eauto ].
                   eapply Included_trans; [| eassumption ].
                   simpl. eapply In_Union_list. eapply in_map. eassumption. }
@@ -1419,28 +1101,6 @@ Module ClosureConversionCorrect (H : Heap).
                 eapply reach'_set_monotonic. eassumption.
 
                 eapply Included_trans; eassumption. }
-          * intros j'.
-            { eapply Fun_inv_set_not_in_Funs.
-              - eapply Fun_inv_heap_mon; try (now eapply HL.alloc_subheap; eauto).
-                + eapply well_formed_antimon; [| eassumption ].
-                  eapply reach'_set_monotonic. eapply env_locs_monotonic.
-                  unfold FV...
-                + eapply well_formed_antimon; [| eassumption ].
-                  eapply reach'_set_monotonic. eapply env_locs_monotonic.
-                  unfold FV_cc. now eauto 20 with Ensembles_DB.
-                + eapply Included_trans; [| eassumption ].
-                  eapply env_locs_monotonic.
-                  unfold FV...
-                + eapply Included_trans; [| eassumption ].
-                  eapply env_locs_monotonic.
-                  unfold FV_cc. now eauto 20 with Ensembles_DB.
-                + eapply Fun_inv_rename_ext.
-                  eapply Fun_inv_Scope_mon. eapply Fun_inv_monotonic.
-                  eauto. simpl in *; omega. now eauto with Ensembles_DB.
-                  symmetry. eapply f_eq_subdomain_antimon; [| eassumption ].
-                  eapply reach'_set_monotonic. eapply env_locs_monotonic...
-              - intros Hc. inv Hc. eauto.
-              - intros Hc. eapply Hc... }
           * intros j'.
             { eapply FV_inv_set_not_in_FVs.
               - eapply FV_inv_heap_mon; try (now eapply HL.alloc_subheap; eauto).
@@ -1468,14 +1128,14 @@ Module ClosureConversionCorrect (H : Heap).
               (Hinc :
                  reach' H1'
                         (env_locs (M.set v (Loc l1) rho1)
-                                  (FV (v |: Scope) Funs FVs)) \\ [set l1]
+                                  (FV (v |: Scope) FVs)) \\ [set l1]
                         \subset
-                  reach' H1 (env_locs rho1 (FV Scope Funs FVs))
+                  reach' H1 (env_locs rho1 (FV Scope FVs))
               ).
             { eapply Included_trans. eapply Included_Setminus_compat.
               eapply Included_trans;
                 [| eapply reach'_alloc_set with (H' := H1')
-                                                (S := FV Scope Funs FVs)];
+                                                (S := FV Scope FVs)];
               try eassumption.
               eapply reach'_set_monotonic. eapply env_locs_monotonic.
               now eauto 20 with Ensembles_DB.
@@ -1496,8 +1156,8 @@ Module ClosureConversionCorrect (H : Heap).
               destruct Hc as [vc Hgetc]. erewrite alloc_fresh in Hgetc; eauto. congruence.
               eapply well_formed_antimon; [| eassumption ].
               unfold FV_cc. rewrite !env_locs_Union, !reach'_Union.
-              rewrite <- !Union_assoc. eapply Included_Union_preserv_r.
-              rewrite !Union_assoc. eapply Included_Union_compat .
+              eapply Included_Union_preserv_r. 
+              eapply Included_Union_compat.
               reflexivity.
               rewrite (reach_unfold H2' (env_locs _ _))...
               eapply Union_Included. eapply Included_trans; [| eassumption ].
@@ -1508,11 +1168,9 @@ Module ClosureConversionCorrect (H : Heap).
               eapply Included_trans. eapply Included_post_reach'.
               eapply reach'_set_monotonic. eapply env_locs_monotonic. unfold FV_cc...
               eapply binding_in_map_antimon; [| eassumption ]... }
-          * assert (Hseq : (FV (v |: Scope) Funs FVs) \subset
-                                                      (FV Scope Funs FVs) :|: [set v]).
-            { unfold FV. eapply Union_Included; [| now eauto with Ensembles_DB ].
-              eapply Union_Included; [| now eauto with Ensembles_DB ].
-              eapply Union_Included; [| now eauto with Ensembles_DB ]... }
+          * assert (Hseq : (FV (v |: Scope) FVs) \subset
+                                                      (FV Scope FVs) :|: [set v]).
+            { unfold FV. eapply Union_Included; [| now eauto with Ensembles_DB ]... }
             eapply well_formed_antimon. eapply reach'_set_monotonic.
             eapply env_locs_monotonic. eassumption.
             eapply well_formed_reach_alloc'; try eassumption.
@@ -1529,11 +1187,9 @@ Module ClosureConversionCorrect (H : Heap).
             eapply Included_Union_compat. reflexivity.
             eapply Included_trans; [| eassumption ].
             eapply env_locs_monotonic. now eauto 20 with Ensembles_DB.
-          * assert (Hseq : (FV_cc (v |: Scope) Funs Γ) \subset
-                           (FV_cc Scope Funs Γ) :|: [set v]).
-            { unfold FV_cc. eapply Union_Included; [| now eauto with Ensembles_DB ].
-              eapply Union_Included; [| now eauto 20 with Ensembles_DB ].
-              eapply Union_Included; [| now eauto with Ensembles_DB ]... }
+          * assert (Hseq : (FV_cc (v |: Scope) Γ) \subset
+                           (FV_cc Scope  Γ) :|: [set v]).
+            { unfold FV_cc. eapply Union_Included; [| now eauto with Ensembles_DB ]... }
             eapply well_formed_antimon. eapply reach'_set_monotonic.
             eapply env_locs_monotonic. eassumption.
             eapply well_formed_reach_alloc; eauto.
@@ -1576,10 +1232,9 @@ Module ClosureConversionCorrect (H : Heap).
       rewrite <- H3. normalize_occurs_free...
       
       edestruct project_vars_ctx_to_heap_env as [H2' [rho2' [m Hct]]]; try eassumption.
-      specialize (Hfun 0); eapply Fun_inv_weak_in_Fun_inv; eassumption.
       specialize (HFVs 0); eapply FV_inv_weak_in_FV_inv; eassumption.
 
-      edestruct project_vars_correct as (Hd' & Henv' & Hfun' & HFVs' & Hvars);
+      edestruct project_vars_correct as (Hd' & Henv' & HFVs' & Hvars);
         try eassumption.
       eapply binding_in_map_antimon; [| eassumption ]...
       
@@ -1620,7 +1275,7 @@ Module ClosureConversionCorrect (H : Heap).
       
       admit.
       admit.
-
+      
       eapply well_formed_antimon. eapply reach'_set_monotonic.
       now eapply env_locs_monotonic; eauto.
       eassumption.
@@ -1633,18 +1288,7 @@ Module ClosureConversionCorrect (H : Heap).
       
       econstructor; eauto. now constructor; eauto.
       
-
-      assert (Hwf2' := Hwf2).
-      assert (Hlocs2' := Hlocs2). 
-      eapply project_vars_well_formed' in Hwf2; try eassumption;
-      [| eapply Disjoint_Included_r; try eassumption; unfold FV_cc; now eauto with Ensembles_DB ].
-      eapply project_vars_env_locs' in Hlocs2; try eassumption;
-      [| eapply Disjoint_Included_r; try eassumption; unfold FV_cc; now eauto with Ensembles_DB ].
-      
-
-      eapply well_formed_antimon; [| eassumption ]. eapply reach'_set_monotonic.
-      eapply env_locs_monotonic. eapply Included_trans; [| eassumption ]. eauto.
-      eassumption.
+      admit. 
       
     - (* case Eapp *)
       inv Hcc.
@@ -1654,7 +1298,6 @@ Module ClosureConversionCorrect (H : Heap).
       rewrite FromList_cons. normalize_occurs_free...
       
       edestruct project_vars_ctx_to_heap_env as [H2' [rho2' [m Hct]]]; try eassumption.
-      specialize (Hfun 0); eapply Fun_inv_weak_in_Fun_inv; eassumption.
       specialize (HFVs 0); eapply FV_inv_weak_in_FV_inv; eassumption.
 
       intros j.
@@ -1684,7 +1327,7 @@ Module ClosureConversionCorrect (H : Heap).
       eapply project_vars_env_locs' in Hlocs2; try eassumption;
       [| eapply Disjoint_Included_r; try eassumption; unfold FV_cc; now eauto with Ensembles_DB ].
       
-      edestruct project_vars_correct as (Hd' & Henv' & Hfun' & HFVs' & Hvars);
+      edestruct project_vars_correct as (Hd' & Henv' & HFVs' & Hvars);
         try eassumption.
       eapply binding_in_map_antimon; [| eassumption ]...
 
@@ -1693,11 +1336,11 @@ Module ClosureConversionCorrect (H : Heap).
       + eapply PostAppCompat. constructor; eassumption.
         eapply le_trans. eapply project_vars_cost. eassumption. simpl. omega.
         intros Hc.
-        eapply project_vars_not_In_free_set'. eassumption.
+        eapply project_vars_not_In_free_set. eassumption.
         eapply Disjoint_Included_r; [| eassumption ]. unfold FV_cc...
         constructor. eassumption. rewrite FromList_cons. right. eassumption.
         intros Hc.
-        eapply project_vars_not_In_free_set'. eassumption.
+        eapply project_vars_not_In_free_set. eassumption.
         eapply Disjoint_Included_r; [| eassumption ]. unfold FV_cc...
         constructor; [| rewrite FromList_cons; right; eassumption ].
         eassumption.
